misc.

coq/SimpleForm/Simplifications/Simplify.v
@@ -1,3 +1,4 @@
+Require Import Koika.KoikaForm.Untyped.UntypedSemantics.
 Require Import Koika.SimpleForm.SimpleFormInterpretation.
 Require Import Koika.SimpleForm.SimpleFormOperations.
 Require Import Koika.BitsToLists.
@@ -29,10 +30,933 @@ Section Simplify.
     -> wt_val (retSig (Sigma ufn)) (sigma ufn vc)
   }.
 
+  Fixpoint simplify_sact (ua: sact) : sact :=
+    match ua with
+    | SIf cond tb fb =>
+      let cond' := simplify_sact cond in
+      match eval_sact_no_vars r sigma cond' with
+      | Some (Bits [true]) => simplify_sact tb
+      | Some (Bits [false]) => simplify_sact fb
+      | _ => SIf cond' (simplify_sact tb) (simplify_sact fb)
+      end
+    | SBinop ufn a1 a2 =>
+      let a1' := simplify_sact a1 in
+      match ufn with
+      | PrimUntyped.UBits2 PrimUntyped.UAnd =>
+        match eval_sact_no_vars r sigma a1' with
+        | Some (Bits [false]) => const_false
+        | Some (Bits [true]) => simplify_sact a2
+        | _ =>
+          let a2' := simplify_sact a2 in
+          match eval_sact_no_vars r sigma a2' with
+          | Some (Bits [false]) => const_false
+          | Some (Bits [true]) => a1'
+          | _ => SBinop ufn a1' a2'
+          end
+        end
+      | PrimUntyped.UBits2 PrimUntyped.UOr =>
+        match eval_sact_no_vars r sigma a1' with
+        | Some (Bits [true]) => const_true
+        | Some (Bits [false]) => simplify_sact a2
+        | _ =>
+          let a2' := simplify_sact a2 in
+          match eval_sact_no_vars r sigma a2' with
+          | Some (Bits [true]) => const_true
+          | Some (Bits [false]) => a1'
+          | _ => SBinop ufn a1' a2'
+          end
+        end
+      | fn =>
+        let a2' := simplify_sact a2 in
+        match eval_sact_no_vars r sigma a1', eval_sact_no_vars r sigma a2' with
+        | Some x, Some y =>
+          match sigma2 fn x y with
+          | Some r => SConst r
+          | None => SBinop ufn a1' a2'
+          end
+        | _, _ => SBinop ufn a1' a2'
+        end
+      end
+    | SUnop ufn a => (* Perhaps not strictly required *)
+      let a := simplify_sact a in
+      (* match ufn with *)
+      (* | PrimUntyped.UBits1 PrimUntyped.UNot => *)
+      (*   match eval_sact_no_vars a with *)
+      (*   | Some (Bits [b]) => SConst (Bits [negb b]) *)
+      (*   | _ => SUnop ufn a *)
+      (*   end *)
+      (* | fn => *)
+        match eval_sact_no_vars r sigma a with
+        | Some x =>
+          match sigma1 ufn x with
+          | Some r => SConst r
+          | None => SUnop ufn a
+          end
+        | None => SUnop ufn a
+        end
+      (* end *)
+    | SExternalCall ufn a => SExternalCall ufn (simplify_sact a)
+    | SVar _ | SReg _ | SConst _ => ua
+    end.
+
+  Definition simplify_vars (v: var_value_map) :=
+    Maps.PTree.map (fun _ '(t, a) => (t, simplify_sact a)) v.
+
   Definition simplify_sf (sf: simple_form) := {|
     final_values := final_values sf;
-    vars := simplify_vars r sigma (vars sf)
+    vars := simplify_vars (vars sf)
   |}.
+
+  Lemma simplify_unop_cases:
+    forall ufn a a',
+    simplify_sact (SUnop ufn a) = a'
+    -> forall ta tr vss, wt_unop ufn ta tr
+    -> wt_sact (Sigma:=Sigma) R vss a ta
+    -> (
+      exists b x,
+      eval_sact_no_vars r sigma (simplify_sact a) = Some b
+      /\ sigma1 ufn b = Some x
+      /\ a' = SConst x)
+    \/ a' = SUnop ufn (simplify_sact a).
+  Proof.
+    intros. simpl in H. simpl.
+    subst. destr. destr.
+    - left. exists v, v0; split; auto.
+    - right; auto.
+    - right; auto.
+  Qed.
+
+  Lemma simplify_bnop_cases:
+    forall ufn a1 a2 a' ,
+    simplify_sact (SBinop ufn a1 a2) = a'
+    -> a' = SBinop ufn (simplify_sact a1) (simplify_sact a2)
+    \/ (ufn = PrimUntyped.UBits2 PrimUntyped.UAnd
+        /\ ((eval_sact_no_vars r sigma (simplify_sact a1) = Some (Bits [true])
+             /\ a' = simplify_sact a2)
+            \/ (eval_sact_no_vars r sigma (simplify_sact a1) = Some (Bits [false])
+                /\ a' = const_false)
+            \/ (eval_sact_no_vars r sigma (simplify_sact a2) = Some (Bits [true])
+                /\ a' = simplify_sact a1)
+            \/ (eval_sact_no_vars r sigma (simplify_sact a2) = Some (Bits [false])
+                /\ a' = const_false)))
+    \/ (ufn = PrimUntyped.UBits2 PrimUntyped.UOr
+        /\ ((eval_sact_no_vars r sigma (simplify_sact a1) = Some (Bits [true])
+             /\ a' = const_true)
+            \/ (eval_sact_no_vars r sigma (simplify_sact a1) = Some (Bits [false])
+                /\ a' = simplify_sact a2)
+            \/ (eval_sact_no_vars r sigma (simplify_sact a2) = Some (Bits [true])
+                /\ a' = const_true)
+            \/ (eval_sact_no_vars r sigma (simplify_sact a2) = Some (Bits [false])
+                /\ a' = simplify_sact a1)))
+  \/ (
+      exists v1 v2 v,
+      eval_sact_no_vars r sigma (simplify_sact a1) = Some v1
+      /\ eval_sact_no_vars r sigma (simplify_sact a2) = Some v2
+      /\ sigma2 ufn v1 v2 = Some v
+      /\ a' = SConst v).
+  Proof.
+    intros. simpl in H. subst.
+    repeat destr; intuition eauto; repeat right; do 3 eexists; repeat split;
+      eauto.
+  Qed.
+
+  Lemma simplify_sact_correct:
+    forall vvs (WTV: wt_vvs R (Sigma:=Sigma) vvs) n a res t,
+    wt_sact (Sigma:=Sigma) R vvs a t
+    -> eval_sact vvs a n = Some res
+    -> eval_sact vvs (simplify_sact a) n = Some res.
+  Proof.
+    induction n; intros a res t WT EVAL; eauto.
+    simpl in EVAL.
+    unfold opt_bind in EVAL.
+    repeat destr_in EVAL; inv EVAL; auto.
+    - simpl. rewrite Heqo; eauto.
+    - inv WT.
+      simpl.
+      destruct (eval_sact_no_vars r sigma (simplify_sact s1)) eqn:?.
+      eapply eval_sact_eval_sact_no_vars in Heqo0; eauto. subst.
+      transitivity (eval_sact vvs (simplify_sact s2) (S n)). reflexivity.
+      exploit IHn. 2: apply H0. eauto. intro ES.
+      exploit (
+        eval_sact_more_fuel (reg_t := reg_t) (ext_fn_t := ext_fn_t)
+        (REnv := REnv)
+      ).
+      apply ES.
+      2: intro ES'; rewrite ES'. lia. eauto.
+      erewrite IHn. 2-3: eauto. simpl.
+      erewrite IHn; eauto.
+    - inv WT.
+      simpl.
+      destruct (eval_sact_no_vars r sigma (simplify_sact s1)) eqn:?.
+      eapply eval_sact_eval_sact_no_vars in Heqo0; eauto. subst.
+      transitivity (eval_sact vvs (simplify_sact s3) (S n)). reflexivity.
+      exploit IHn. 2: apply H0. eauto. intro ES.
+      exploit (
+        eval_sact_more_fuel (reg_t := reg_t) (ext_fn_t := ext_fn_t)
+        (REnv := REnv)
+      ).
+      apply ES.
+      2: intro ES'; rewrite ES'. lia. eauto.
+      erewrite IHn. 2-3: eauto. simpl.
+      erewrite IHn; eauto.
+    - inv WT.
+      edestruct (simplify_unop_cases ufn1 s _ eq_refl) as
+        [(b & vv & EQ & ESNV & EQ')|EQ]; eauto.
+      + rewrite EQ'. simpl.
+        exploit (
+          eval_sact_eval_sact_no_vars (reg_t := reg_t) (ext_fn_t := ext_fn_t)
+          (REnv := REnv)
+        ).
+        2: eauto. eapply IHn. eauto. eauto.
+        intros ->.
+        simpl. auto.
+      + rewrite EQ. simpl. erewrite IHn; simpl; eauto.
+    - inv WT.
+      exploit (
+        eval_sact_wt (reg_t := reg_t) (ext_fn_t := ext_fn_t) (REnv := REnv)
+      ).
+      5: apply Heqo. all: eauto.
+      exploit (
+        eval_sact_wt (reg_t := reg_t) (ext_fn_t := ext_fn_t) (REnv := REnv)
+      ).
+      5: apply Heqo0. all: eauto.
+      intros WTv2 WTv1.
+      exploit Wt.wt_binop_sigma1. eauto. eauto. eauto. eauto. intro WTres.
+      eapply IHn in Heqo; eauto.
+      eapply IHn in Heqo0; eauto.
+      destruct (simplify_bnop_cases ufn2 s1 s2 _ eq_refl) as
+        [EQ|[(ufneq & [(ESNV & EQ)|[(ESNV & EQ)|[(ESNV & EQ)|(ESNV & EQ)]]])
+            |[(ufneq & [(ESNV & EQ)|[(ESNV & EQ)|[(ESNV & EQ)|(ESNV & EQ)]]])|
+        (v1 & v2 & vv & ESNV1 & ESNV2 & SIGMA & EQ)]]]; rewrite EQ; clear EQ.
+      + simpl. rewrite Heqo, Heqo0.  reflexivity.
+      + exploit (
+          eval_sact_eval_sact_no_vars (reg_t := reg_t) (ext_fn_t := ext_fn_t)
+          (REnv := REnv)
+        ).
+        apply Heqo. apply ESNV. intros ->.
+        inv WTv1. inv H6.
+        apply Sact.wt_val_bool in WTv2.
+        apply Sact.wt_val_bool in WTres.
+        destruct WTv2, WTres. subst.
+        unfold eval_sact.
+        erewrite eval_sact_more_fuel. 2: eauto. simpl. auto. lia.
+      + exploit (
+          eval_sact_eval_sact_no_vars (reg_t := reg_t) (ext_fn_t := ext_fn_t)
+          (REnv := REnv)
+        ). apply Heqo. apply ESNV. intros ->.
+        inv WTv1. inv H6.
+        apply Sact.wt_val_bool in WTv2.
+        apply Sact.wt_val_bool in WTres.
+        destruct WTv2, WTres. subst.
+        simpl. auto.
+      + exploit (
+          eval_sact_eval_sact_no_vars (reg_t := reg_t) (ext_fn_t := ext_fn_t)
+          (REnv := REnv)
+        ). eauto. apply ESNV. eauto. intros ->.
+        inv WTv2. inv H6.
+        apply Sact.wt_val_bool in WTv1.
+        apply Sact.wt_val_bool in WTres.
+        destruct WTv1, WTres. subst.
+        unfold eval_sact.
+        erewrite eval_sact_more_fuel. 2: eauto. simpl.
+        rewrite andb_true_r; auto. lia.
+      + exploit (
+          eval_sact_eval_sact_no_vars (reg_t := reg_t) (ext_fn_t := ext_fn_t)
+          (REnv := REnv)
+        ). eauto. apply ESNV. eauto. intros ->.
+        inv WTv2. inv H6.
+        apply Sact.wt_val_bool in WTv1.
+        apply Sact.wt_val_bool in WTres.
+        destruct WTv1, WTres. subst.
+        simpl. rewrite andb_false_r; auto.
+      + exploit (
+          eval_sact_eval_sact_no_vars (reg_t := reg_t) (ext_fn_t := ext_fn_t)
+          (REnv := REnv)
+        ). 2: apply ESNV. eauto. intros ->.
+        inv WTv1. inv H6.
+        apply Sact.wt_val_bool in WTv2.
+        apply Sact.wt_val_bool in WTres.
+        destruct WTv2, WTres. subst. simpl; auto.
+      + exploit (
+          eval_sact_eval_sact_no_vars (reg_t := reg_t) (ext_fn_t := ext_fn_t)
+          (REnv := REnv)
+        ). 2: apply ESNV. eauto. intros ->.
+        inv WTv1. inv H6.
+        apply Sact.wt_val_bool in WTv2.
+        apply Sact.wt_val_bool in WTres.
+        destruct WTv2, WTres. subst.
+        unfold eval_sact.
+        erewrite eval_sact_more_fuel. 2: eauto. simpl. auto. lia.
+      + exploit (
+          eval_sact_eval_sact_no_vars (reg_t := reg_t) (ext_fn_t := ext_fn_t)
+          (REnv := REnv)
+        ). 2: apply ESNV. eauto. intros ->.
+        inv WTv2. inv H6.
+        apply Sact.wt_val_bool in WTv1.
+        apply Sact.wt_val_bool in WTres.
+        destruct WTv1, WTres. subst. simpl. rewrite orb_true_r; auto.
+      + exploit (
+          eval_sact_eval_sact_no_vars (reg_t := reg_t) (ext_fn_t := ext_fn_t)
+          (REnv := REnv)
+        ). 2: apply ESNV. eauto. intros ->.
+        inv WTv2. inv H6.
+        apply Sact.wt_val_bool in WTv1.
+        apply Sact.wt_val_bool in WTres.
+        destruct WTv1, WTres. subst.
+        unfold eval_sact.
+        erewrite eval_sact_more_fuel. 2: eauto. simpl.
+        rewrite orb_false_r; auto. lia.
+      + exploit (
+          eval_sact_eval_sact_no_vars (reg_t := reg_t) (ext_fn_t := ext_fn_t)
+          (REnv := REnv)
+        ). 2: apply ESNV1. eauto. intros ->.
+        exploit (
+          eval_sact_eval_sact_no_vars (reg_t := reg_t) (ext_fn_t := ext_fn_t)
+          (REnv := REnv)
+        ). 2: apply ESNV2. eauto. intros ->.
+        rewrite H0 in SIGMA. inv SIGMA. simpl. eauto.
+    - simpl. inv WT;  erewrite IHn; simpl; eauto.
+  Qed.
+
+  Lemma wt_simplify_sact:
+    forall vss a t,
+    wt_sact R (Sigma:=Sigma) vss a t
+    -> wt_sact R (Sigma:=Sigma) vss (simplify_sact a) t.
+  Proof.
+    induction 1; simpl; intros; eauto.
+    - econstructor; eauto.
+    - econstructor; eauto.
+    - destr.
+      exploit (
+        eval_sact_no_vars_wt
+          (reg_t := reg_t) (ext_fn_t := ext_fn_t) (REnv := REnv)
+      ).
+      eauto. eauto. 2: eauto. eauto.
+      intro WT. apply Sact.wt_val_bool in WT. destruct WT; subst.
+      destr.
+      econstructor; eauto.
+    - assert (
+        wt_sact
+          (Sigma:=Sigma) R vss
+          match eval_sact_no_vars r sigma (simplify_sact a) with
+          | Some x =>
+            match sigma1 ufn x with
+            | Some r => SConst r
+            | None => SUnop ufn (simplify_sact a)
+            end
+          | None => SUnop ufn (simplify_sact a)
+          end t'
+      ). {
+        destr.
+        exploit (
+          eval_sact_no_vars_wt
+            (reg_t := reg_t) (ext_fn_t := ext_fn_t) (REnv := REnv)
+        ).
+        eauto. eauto. 2: eauto. eauto.
+        intro WT.
+        destr.
+        econstructor; eauto.
+        eapply Wt.wt_unop_sigma1; eauto.
+        econstructor; eauto.
+        econstructor; eauto.
+      }
+      destr; auto.
+    - assert ( wt_sact (Sigma:=Sigma) R vss
+                 match eval_sact_no_vars r sigma (simplify_sact a1) with
+                 | Some x =>
+                     match eval_sact_no_vars r sigma (simplify_sact a2) with
+                     | Some y => match sigma2 ufn x y with
+                                 | Some r0 => SConst r0
+                                 | None => SBinop ufn (simplify_sact a1) (simplify_sact a2)
+                                 end
+                     | None => SBinop ufn (simplify_sact a1) (simplify_sact a2)
+                     end
+                 | None => SBinop ufn (simplify_sact a1) (simplify_sact a2)
+                 end t').
+      {
+        destr.
+        2: econstructor; eauto.
+        destr.
+        2: econstructor; eauto.
+        exploit (
+          eval_sact_no_vars_wt
+            (reg_t := reg_t) (ext_fn_t := ext_fn_t) (REnv := REnv)
+        ). eauto. eauto.
+        2: apply Heqo. eauto.
+        intro WT1.
+        exploit (
+          eval_sact_no_vars_wt
+            (reg_t := reg_t) (ext_fn_t := ext_fn_t) (REnv := REnv)
+        ). eauto. eauto.
+        2: apply Heqo0. eauto.
+        intro WT2.
+        destr.
+        2: econstructor; eauto.
+        econstructor.
+        eapply Wt.wt_binop_sigma1; eauto.
+      }
+      destr; auto.
+      destr; auto.
+      + clear H2. inv H1.
+        destr.
+        exploit (
+          eval_sact_no_vars_wt
+            (reg_t := reg_t) (ext_fn_t := ext_fn_t) (REnv := REnv)
+        ). eauto. eauto.
+        apply IHwt_sact1. eauto.
+        intro WT1. inv WT1.
+        destruct (eval_sact_no_vars r sigma (simplify_sact a2)) eqn:?.
+        exploit (
+          eval_sact_no_vars_wt
+            (reg_t := reg_t) (ext_fn_t := ext_fn_t) (REnv := REnv)
+        ). eauto. eauto.
+        apply IHwt_sact2. eauto.
+        intro WT2. inv WT2.
+        destr. destr. econstructor; eauto. econstructor; eauto.
+        simpl in H2; lia.
+        destruct bs0. simpl in H2; lia. simpl in H2. destruct l.
+        destr; eauto. constructor. constructor. auto.
+        destruct bs0. simpl in H2; lia. simpl in H2.
+        repeat destr; eauto; econstructor; eauto; constructor; auto.
+        repeat destr; repeat econstructor; eauto.
+        repeat destr; repeat econstructor; eauto.
+        subst.
+        exploit (
+          eval_sact_no_vars_wt
+            (reg_t := reg_t) (ext_fn_t := ext_fn_t) (REnv := REnv)
+        ). eauto. eauto.
+        apply IHwt_sact2. eauto.
+        intro WT2. inv WT2.
+        auto.
+      + clear H2. inv H1.
+        destr.
+        exploit (
+          eval_sact_no_vars_wt
+            (reg_t := reg_t) (ext_fn_t := ext_fn_t) (REnv := REnv)
+        ). eauto. eauto.
+        apply IHwt_sact1. eauto.
+        intro WT1. inv WT1.
+        destruct (eval_sact_no_vars r sigma (simplify_sact a2)) eqn:?.
+        exploit (
+          eval_sact_no_vars_wt
+            (reg_t := reg_t) (ext_fn_t := ext_fn_t) (REnv := REnv)
+        ). eauto. eauto.
+        apply IHwt_sact2. eauto.
+        intro WT2. inv WT2.
+        destr. destr. econstructor; eauto. econstructor; eauto.
+        simpl in H2; lia.
+        destruct bs0. simpl in H2; lia. simpl in H2. destruct l.
+        destr; eauto. constructor. constructor. auto.
+        destruct bs0. simpl in H2; lia. simpl in H2.
+        repeat destr; eauto; econstructor; eauto; constructor; auto.
+        repeat destr; repeat econstructor; eauto.
+        repeat destr; repeat econstructor; eauto.
+        subst.
+        exploit (
+          eval_sact_no_vars_wt
+            (reg_t := reg_t) (ext_fn_t := ext_fn_t) (REnv := REnv)
+        ). eauto. eauto.
+        apply IHwt_sact2. eauto.
+        intro WT2. inv WT2.
+        auto.
+    - econstructor; eauto.
+    - econstructor; eauto.
+  Qed.
+
+  Lemma simplify_sact_wt_sact_ok':
+    forall vvs a t (WTS: wt_sact (Sigma := Sigma) R vvs a t),
+    wt_sact (Sigma := Sigma) R vvs (simplify_sact a) t.
+  Proof. apply wt_simplify_sact. Qed.
+
+  Lemma simplify_vars_wt_sact_ok:
+    forall vvs s t (WTS: wt_sact (Sigma := Sigma) R (simplify_vars vvs) s t),
+    wt_sact (Sigma := Sigma) R vvs s t.
+  Proof.
+    intros.
+    induction WTS; try (econstructor; eauto; fail).
+    unfold simplify_vars in H.
+    rewrite Maps.PTree.gmap in H. unfold option_map in H.
+    destr_in H. destruct p.
+    - apply Some_inj in H. apply pair_inj in H. destruct H. subst.
+      econstructor. eauto.
+    - easy.
+  Qed.
+
+  Lemma simplify_vars_wt_sact_ok':
+    forall vvs s t (WTS: wt_sact (Sigma := Sigma) R vvs s t),
+    wt_sact (Sigma := Sigma) R (simplify_vars vvs) s t.
+  Proof.
+    intros.
+    induction WTS; econstructor; eauto.
+    unfold simplify_vars.
+    setoid_rewrite Maps.PTree.gmap.
+    unfold option_map. setoid_rewrite H. easy.
+  Qed.
+
+  Lemma simplify_vars_get_ok:
+    forall vvs x t a (GET: Maps.PTree.get x (simplify_vars vvs) = Some (t, a)),
+    exists a', Maps.PTree.get x vvs = Some (t, a').
+  Proof.
+    intros. unfold simplify_vars in GET.
+    rewrite Maps.PTree.gmap in GET. unfold option_map in GET.
+    repeat (destr_in GET); inv GET; eauto.
+  Qed.
+
+  Lemma simplify_vars_get_ok':
+    forall vvs x t a (GET: Maps.PTree.get x vvs = Some (t, a)),
+    Maps.PTree.get x (simplify_vars vvs) = Some (t, simplify_sact a).
+  Proof.
+    intros. unfold simplify_vars.
+    rewrite Maps.PTree.gmap. unfold option_map.
+    setoid_rewrite GET. eauto.
+  Qed.
+
+  Lemma simplify_vars_wtvvs_ok':
+    forall vvs (WTVVS: wt_vvs (Sigma := Sigma) R vvs),
+    wt_vvs (Sigma := Sigma) R (simplify_vars vvs).
+  Proof.
+    intros. unfold wt_vvs. intros.
+    apply simplify_vars_wt_sact_ok'.
+    unfold simplify_vars in H.
+    rewrite Maps.PTree.gmap in H. unfold option_map in H.
+    destr_in H. destruct p.
+    - apply Some_inj in H. apply pair_inj in H. destruct H. subst t0.
+      inv H0. apply simplify_sact_wt_sact_ok'; eauto.
+    - easy.
+  Qed.
+
+  Lemma simplify_sact_reachable_vars_ok:
+    forall vvs s v (RV: reachable_var vvs (simplify_sact s) v),
+    reachable_var vvs s v.
+  Proof.
+    intros.
+    induction s; simpl in *; eauto.
+    - repeat (destr_in RV); eauto;
+        try (
+          inv RV;
+          try (eapply reachable_var_if_cond; eauto; fail);
+          try (eapply reachable_var_if_true; eauto; fail);
+          try (eapply reachable_var_if_false; eauto; fail);
+          fail); subst.
+      + eapply IHs2 in RV. eapply reachable_var_if_true; eauto.
+      + eapply IHs3 in RV. eapply reachable_var_if_false; eauto.
+    - repeat (destr_in RV); econstructor; inv RV; eauto.
+    - repeat (destr_in RV);
+      try (eapply reachable_var_binop1; eauto; fail);
+      try (eapply reachable_var_binop2; eauto; fail);
+      try (
+        inv RV;
+        try (eapply reachable_var_binop1; eauto; fail);
+        try (eapply reachable_var_binop2; eauto; fail);
+        fail
+      );
+      subst.
+    - inv RV. econstructor. eauto.
+  Qed.
+
+  Lemma simplify_sact_interp_sact_ok':
+    forall a v vvs (WTVVS: wt_vvs (Sigma := Sigma) R vvs) t
+      (WTS: wt_sact (Sigma := Sigma) R vvs a t)
+      (VVSSV: vvs_smaller_variables vvs),
+    interp_sact (sigma := sigma) REnv r vvs a v
+    -> interp_sact (sigma := sigma) REnv r vvs (simplify_sact a) v.
+  Proof.
+    intros.
+    eapply interp_sact_do_eval_sact in H; eauto.
+    unfold do_eval_sact in H.
+    eapply eval_sact_interp_sact.
+    erewrite simplify_sact_correct; eauto.
+  Qed.
+
+  Lemma simplify_sact_var_in_sact_ok':
+    forall s v (VIS: var_in_sact (simplify_sact s) v),
+    var_in_sact s v.
+  Proof.
+    intros.
+    induction s; try (eauto; fail).
+    - simpl in VIS. repeat (destr_in VIS); try (
+        inv VIS; try (apply var_in_if_cond; eauto; fail);
+        try (apply var_in_if_true; eauto; fail);
+        try (apply var_in_if_false; eauto; fail);
+        fail).
+      + apply var_in_if_true; eauto.
+      + apply var_in_if_false; eauto.
+    - simpl in VIS. repeat (destr_in VIS);
+        (econstructor; eapply IHs; inv VIS; easy).
+    - simpl in VIS. destr_in VIS;
+      try (
+        inv VIS;
+        try (apply var_in_sact_binop_1; eauto; fail);
+        try (apply var_in_sact_binop_2; eauto; fail);
+        fail).
+      repeat (destr_in VIS);
+        try (apply var_in_sact_binop_1; eauto; fail);
+        try (apply var_in_sact_binop_2; eauto; fail);
+        try (
+          inv VIS; try (apply var_in_sact_binop_1; eauto; fail);
+          try (apply var_in_sact_binop_2; eauto; fail); fail).
+      repeat (destr_in VIS);
+        try (apply var_in_sact_binop_1; eauto; fail);
+        try (apply var_in_sact_binop_2; eauto; fail);
+        try (
+          inv VIS; try (apply var_in_sact_binop_1; eauto; fail);
+          try (apply var_in_sact_binop_2; eauto; fail); fail).
+      repeat (destr_in VIS);
+        try (apply var_in_sact_binop_1; eauto; fail);
+        try (apply var_in_sact_binop_2; eauto; fail);
+        try (
+          inv VIS; try (apply var_in_sact_binop_1; eauto; fail);
+          try (apply var_in_sact_binop_2; eauto; fail); fail).
+      repeat (destr_in VIS);
+        try (apply var_in_sact_binop_1; eauto; fail);
+        try (apply var_in_sact_binop_2; eauto; fail);
+        try (
+          inv VIS; try (apply var_in_sact_binop_1; eauto; fail);
+          try (apply var_in_sact_binop_2; eauto; fail); fail).
+    - inv VIS. econstructor. eauto.
+  Qed.
+
+  Lemma simplify_vars_vvssv_ok':
+    forall vvs (VVSSV: vvs_smaller_variables vvs),
+    vvs_smaller_variables (simplify_vars vvs).
+  Proof.
+    intros.
+    unfold vvs_smaller_variables in *. intros.
+    unfold simplify_vars in H.
+    rewrite Maps.PTree.gmap in H. unfold option_map in H.
+    destr_in H. destruct p.
+    - apply Some_inj in H. apply pair_inj in H. destruct H. subst t0.
+      eapply VVSSV; eauto. inv H1.
+      apply simplify_sact_var_in_sact_ok'. eauto.
+    - easy.
+  Qed.
+
+  Lemma simplify_vars_interp_sact_ok':
+    forall vvs a v (WTVVS: wt_vvs (Sigma := Sigma) R vvs)
+      (VVSSV: vvs_smaller_variables vvs)
+      (EV_INIT: interp_sact (sigma := sigma) REnv r vvs a v),
+    interp_sact (sigma := sigma) REnv r (simplify_vars vvs) a v.
+  Proof.
+    intros.
+    induction EV_INIT; try (econstructor; eauto; fail).
+    econstructor.
+    - unfold simplify_vars. setoid_rewrite Maps.PTree.gmap.
+      unfold option_map. setoid_rewrite H.
+      f_equal.
+    - eapply simplify_sact_interp_sact_ok'; eauto.
+      + apply simplify_vars_wtvvs_ok'. eauto.
+      + apply simplify_vars_wt_sact_ok'. eauto.
+      + apply simplify_vars_vvssv_ok'. eauto.
+  Qed.
+
+  Lemma simplify_vars_ok:
+    forall
+      fuel vvs a res (EV_INIT: eval_sact vvs a fuel = Some res)
+      (WTVVS: wt_vvs (Sigma := Sigma) R vvs) t
+      (WTS: wt_sact (Sigma := Sigma) R vvs a t),
+    eval_sact (simplify_vars vvs) a fuel = Some res.
+  Proof.
+    induction fuel; simpl; intros; eauto.
+    Transparent eval_sact.
+    destruct a; simpl in *.
+    - unfold opt_bind in EV_INIT. repeat destr_in EV_INIT; inv EV_INIT.
+      setoid_rewrite PTree.gmap. setoid_rewrite Heqo. simpl.
+      erewrite IHfuel. eauto. eapply simplify_sact_correct; eauto. auto.
+      eapply wt_simplify_sact; eauto.
+    - congruence.
+    - unfold opt_bind in EV_INIT. destr_in EV_INIT; inv EV_INIT.
+      erewrite IHfuel. 2: eauto. simpl.
+      destr_in H0; inv H0.
+      destr_in H1; inv H1.
+      destr_in H0; inv H0.
+      rewrite H1.
+      inv WTS.
+      destr_in H1; (erewrite IHfuel; eauto).
+      auto. inv WTS. eauto.
+    - unfold opt_bind in EV_INIT. destr_in EV_INIT; inv EV_INIT.
+      inv WTS.
+      erewrite IHfuel. 2: eauto. simpl. auto. auto. eauto.
+    - unfold opt_bind in EV_INIT. destr_in EV_INIT; inv EV_INIT.
+      destr_in H0; inv H0.
+      inv WTS.
+      erewrite IHfuel; eauto.
+      erewrite IHfuel; eauto. simpl. auto.
+    - unfold opt_bind in EV_INIT. destr_in EV_INIT; inv EV_INIT.
+      inv WTS.
+      erewrite IHfuel. 2: eauto. simpl. auto. auto. eauto.
+    - auto.
+  Qed.
+
+  Lemma simplify_sact_interp_sact_ok:
+    forall
+      vvs (WTVVS: wt_vvs (Sigma := Sigma) R vvs)
+      (VVSSV: vvs_smaller_variables vvs) a v
+      (EV_INIT: interp_sact (sigma := sigma) REnv r vvs (simplify_sact a) v)
+      t (WTS: wt_sact (Sigma := Sigma) R vvs a t),
+    interp_sact (sigma := sigma) REnv r vvs a v.
+  Proof.
+    induction a; simpl; intros; eauto; inv WTS.
+    - destr_in EV_INIT.
+      exploit (
+        eval_sact_no_vars_wt
+          (reg_t := reg_t) (ext_fn_t := ext_fn_t) (REnv := REnv)
+      ). 4: apply Heqo. all: eauto.
+      apply wt_simplify_sact. eauto. intro WT. apply Sact.wt_val_bool in WT.
+      destruct WT; subst.
+      econstructor. eapply eval_sact_no_vars_interp in Heqo.
+      eapply IHa1 in Heqo. eauto. eauto. destr; eauto.
+      inv EV_INIT.
+      econstructor; eauto.
+      destr; eauto.
+    - destr_in EV_INIT.
+      destr_in EV_INIT.
+      + inv EV_INIT.
+        econstructor; eauto.
+        eapply eval_sact_no_vars_interp in Heqo; eauto.
+      + inv EV_INIT.
+        econstructor; eauto.
+      + inv EV_INIT.
+        econstructor; eauto.
+    - destruct (eval_sact_no_vars r sigma (simplify_sact a1)) eqn:?.
+      exploit (
+        eval_sact_no_vars_interp (reg_t := reg_t) (ext_fn_t := ext_fn_t)
+          (REnv := REnv)
+      ).
+      apply Heqo. intro IS1.
+      destruct (eval_sact_no_vars r sigma (simplify_sact a2)) eqn:?.
+      exploit (
+        eval_sact_no_vars_interp (reg_t := reg_t) (ext_fn_t := ext_fn_t)
+          (REnv := REnv)
+      ).
+      apply Heqo0. intro IS2.
+      + destr_in EV_INIT.
+        destr_in EV_INIT; inv EV_INIT.
+        econstructor; eauto.
+        econstructor; eauto.
+        econstructor; eauto.
+        assert (interp_sact (sigma:=sigma) REnv r vvs match sigma2 (PrimUntyped.UBits2 fn) v0 v1 with
+                                        | Some r => SConst r
+                                        | None => SBinop (PrimUntyped.UBits2 fn) (simplify_sact a1) (simplify_sact a2)
+                                        end v ->
+                sigma2 (PrimUntyped.UBits2 fn) v0 v1 = Some v
+               ).
+        clear EV_INIT.
+        intros EV.
+        destr_in EV. inv EV. auto. inv EV.
+        generalize (interp_sact_determ _ _ _ _ _ IS1 _ H3).
+        generalize (interp_sact_determ _ _ _ _ _ IS2 _ H7). congruence.
+        destr_in EV_INIT; auto.
+        simpl.
+        inv H5.
+        exploit @interp_sact_wt. eauto. eauto. eauto. auto. apply vvs_range_max_var. apply H2. eauto.
+        exploit @interp_sact_wt. eauto. eauto. eauto. auto. apply vvs_range_max_var. apply H4. eauto.
+        intros WT2 WT1. inv WT2; inv WT1. simpl in *.
+        destr_in EV_INIT. destruct bs; [|simpl in H1; lia].
+        inv EV_INIT.
+        generalize (interp_sact_determ _ _ _ _ _ IS1 _ H6).
+        generalize (interp_sact_determ _ _ _ _ _ IS2 _ H8).
+        intros. subst. simpl in H9. inv H9. reflexivity.
+        destruct bs; [simpl in H1; lia|].
+        destruct l, bs; try (simpl in H1; lia).
+        subst. simpl in *.
+        destr_in EV_INIT. simpl.
+        generalize (interp_sact_determ _ _ _ _ _ IS2 _ EV_INIT). congruence. inv EV_INIT. reflexivity.
+        assert ( interp_sact (sigma:=sigma) REnv r vvs
+                   (SBinop (PrimUntyped.UBits2 PrimUntyped.UAnd) (simplify_sact a1) (simplify_sact a2)) v).
+        repeat destr_in EV_INIT; eauto. clear EV_INIT. inv H0.
+        generalize (interp_sact_determ _ _ _ _ _ IS1 _ H7).
+        generalize (interp_sact_determ _ _ _ _ _ IS2 _ H9). intros; subst.
+        simpl in H10. inv H10. simpl. auto.
+        simpl.
+        inv H5.
+        exploit @interp_sact_wt. eauto. eauto. eauto. auto. apply vvs_range_max_var. apply H2. eauto.
+        exploit @interp_sact_wt. eauto. eauto. eauto. auto. apply vvs_range_max_var. apply H4. eauto.
+        intros WT2 WT1. inv WT2; inv WT1. simpl in *.
+        destr_in EV_INIT. destruct bs; [|simpl in H1; lia].
+        inv EV_INIT.
+        generalize (interp_sact_determ _ _ _ _ _ IS1 _ H6).
+        generalize (interp_sact_determ _ _ _ _ _ IS2 _ H8).
+        intros. subst. simpl in H9. inv H9. reflexivity.
+        destruct bs; [simpl in H1; lia|].
+        destruct l, bs; try (simpl in H1; lia).
+        subst. simpl in *.
+        destr_in EV_INIT. simpl. inv EV_INIT. auto. simpl.
+        generalize (interp_sact_determ _ _ _ _ _ IS2 _ EV_INIT). congruence.
+        assert (interp_sact (sigma:=sigma) REnv r vvs
+                   (SBinop (PrimUntyped.UBits2 PrimUntyped.UOr) (simplify_sact a1) (simplify_sact a2)) v).
+        repeat destr_in EV_INIT; eauto. clear EV_INIT. inv H0.
+        generalize (interp_sact_determ _ _ _ _ _ IS1 _ H7).
+        generalize (interp_sact_determ _ _ _ _ _ IS2 _ H9). intros; subst.
+        simpl in H10. inv H10. simpl. auto.
+        destr_in EV_INIT; auto.
+        econstructor. eauto. eauto.
+        inv EV_INIT. auto.
+        inv EV_INIT.
+        generalize (interp_sact_determ _ _ _ _ _ IS1 _ H3).
+        generalize (interp_sact_determ _ _ _ _ _ IS2 _ H7). intros; subst.
+        econstructor; eauto.
+        destr_in EV_INIT; auto.
+        econstructor. eauto. eauto.
+        inv EV_INIT. auto.
+        inv EV_INIT.
+        generalize (interp_sact_determ _ _ _ _ _ IS1 _ H3).
+        generalize (interp_sact_determ _ _ _ _ _ IS2 _ H7). intros; subst.
+        econstructor; eauto.
+      + destr_in EV_INIT. inv EV_INIT.
+        * generalize (interp_sact_determ _ _ _ _ _ IS1 _ H3). intro; subst.
+          econstructor; eauto.
+        * assert (interp_sact (sigma:=sigma) REnv r vvs (SBinop (PrimUntyped.UBits2 fn) (simplify_sact a1) (simplify_sact a2)) v ->
+                  interp_sact (sigma:=sigma) REnv r vvs (SBinop (PrimUntyped.UBits2 fn) a1 a2) v
+                 ).
+          clear EV_INIT.
+          intro IS. inv IS.
+          generalize (interp_sact_determ _ _ _ _ _ IS1 _ H3). intro; subst.
+          econstructor; eauto.
+          repeat destr_in EV_INIT; eauto.
+          clear H.
+          inv H5. econstructor; eauto.
+          exploit @interp_sact_wt. eauto. eauto. eauto. auto. apply vvs_range_max_var. apply H4. eauto.
+          intro A; inv A.
+          exploit @interp_sact_wt. eauto. eauto. eauto. auto. apply vvs_range_max_var. apply H2. eauto.
+          intro A; inv A.
+          simpl in H1. destruct bs; simpl in H1; try lia. destruct bs; simpl in H1; try lia.
+          simpl. auto.
+          clear H.
+          inv H5. inv EV_INIT.
+          exploit @wt_sact_interp. eauto. eauto. eauto. eauto. apply vvs_range_max_var. apply H4. intros (v2 & IS2 & WT2). inv WT2.
+          econstructor; eauto.
+          exploit @interp_sact_wt. eauto. eauto. eauto. auto. apply vvs_range_max_var. apply H2. eauto.
+          intro A; inv A.
+          simpl in H1. destruct bs; simpl in H1; try lia. destruct bs; simpl in H1; try lia.
+          simpl. auto.
+          clear H.
+          inv H5. inv EV_INIT.
+          exploit @wt_sact_interp. eauto. eauto. eauto. eauto. apply vvs_range_max_var. apply H4. intros (v2 & IS2 & WT2). inv WT2.
+          econstructor; eauto.
+          exploit @interp_sact_wt. eauto. eauto. eauto. auto. apply vvs_range_max_var. apply H2. eauto.
+          intro A; inv A.
+          simpl in H1. destruct bs; simpl in H1; try lia. destruct bs; simpl in H1; try lia.
+          simpl. auto.
+          clear H.
+          inv H5. econstructor; eauto.
+          exploit @interp_sact_wt. eauto. eauto. eauto. auto. apply vvs_range_max_var. apply H4. eauto.
+          intro A; inv A.
+          exploit @interp_sact_wt. eauto. eauto. eauto. auto. apply vvs_range_max_var. apply H2. eauto.
+          intro A; inv A.
+          simpl in H1. destruct bs; simpl in H1; try lia. destruct bs; simpl in H1; try lia.
+          simpl. auto.
+        * inv EV_INIT. generalize (interp_sact_determ _ _ _ _ _ IS1 _ H3). intro; subst.
+          econstructor; eauto.
+        * inv EV_INIT. generalize (interp_sact_determ _ _ _ _ _ IS1 _ H3). intro; subst.
+          econstructor; eauto.
+      + assert (interp_sact (sigma:=sigma) REnv r vvs (SBinop ufn2 (simplify_sact a1) (simplify_sact a2)) v ->
+                interp_sact (sigma:=sigma) REnv r vvs (SBinop ufn2 a1 a2) v
+               ).
+        {
+          clear EV_INIT.
+          intro IS. inv IS.
+          econstructor; eauto.
+        }
+        destr_in EV_INIT; auto.
+        repeat destr_in EV_INIT; auto; clear H.
+        econstructor; eauto.
+        eapply IHa2.
+        eapply eval_sact_no_vars_interp. eauto. eauto.
+        exploit (
+          eval_sact_no_vars_wt
+            (reg_t := reg_t)  (ext_fn_t := ext_fn_t) (REnv := REnv)
+        ).
+        4: apply Heqo0. all: eauto. eapply wt_simplify_sact; eauto.
+        exploit @interp_sact_wt. eauto. eauto. eauto. eauto. apply vvs_range_max_var. apply H2. eauto.
+        intros WT1 WT2. inv H5. inv WT2. inv WT1.
+        destruct bs; simpl in H0; try lia.
+        destruct bs; simpl in H0; try lia.
+        simpl. rewrite andb_true_r. auto.
+        exploit @wt_sact_interp. eauto. eauto. eauto. eauto. apply vvs_range_max_var. apply H2. intros (vv1 & IS1 & WT1).
+        econstructor; eauto.
+        eapply IHa2.
+        eapply eval_sact_no_vars_interp. eauto. eauto.
+        exploit (
+          eval_sact_no_vars_wt
+            (reg_t := reg_t)  (ext_fn_t := ext_fn_t) (REnv := REnv)
+        ).
+        4: apply Heqo0. all: eauto. eapply wt_simplify_sact; eauto.
+        intros WT2. inv H5. inv WT2. inv WT1.
+        destruct bs; simpl in H0; try lia.
+        destruct bs; simpl in H0; try lia.
+        simpl. rewrite andb_false_r. inv EV_INIT. auto.
+        exploit @wt_sact_interp. eauto. eauto. eauto. eauto. apply vvs_range_max_var. apply H2. intros (vv1 & IS1 & WT1).
+        econstructor; eauto.
+        eapply IHa2.
+        eapply eval_sact_no_vars_interp. eauto. eauto.
+        exploit (
+          eval_sact_no_vars_wt
+            (reg_t := reg_t)  (ext_fn_t := ext_fn_t) (REnv := REnv)
+        ).
+        4: apply Heqo0. all: eauto. eapply wt_simplify_sact; eauto.
+        intros WT2. inv H5. inv WT2. inv WT1.
+        destruct bs; simpl in H0; try lia.
+        destruct bs; simpl in H0; try lia.
+        simpl. rewrite orb_true_r. inv EV_INIT. auto.
+        econstructor; eauto.
+        eapply IHa2.
+        eapply eval_sact_no_vars_interp. eauto. eauto.
+        exploit (
+          eval_sact_no_vars_wt
+            (reg_t := reg_t)  (ext_fn_t := ext_fn_t) (REnv := REnv)
+        ).
+        4: apply Heqo0. all: eauto. eapply wt_simplify_sact; eauto.
+        exploit @interp_sact_wt. eauto. eauto. eauto. eauto. apply vvs_range_max_var. apply H2. eauto.
+        intros WT1 WT2. inv H5. inv WT2. inv WT1.
+        destruct bs; simpl in H0; try lia.
+        destruct bs; simpl in H0; try lia.
+        simpl. rewrite orb_false_r. auto.
+    - inv EV_INIT. econstructor; eauto.
+  Qed.
+
+  Lemma simplify_vars_interp_sact_ok:
+    forall vvs
+           (WTVVS: wt_vvs (Sigma := Sigma) R vvs)
+           (VVSSV: vvs_smaller_variables vvs)
+           a v
+           (EV_INIT: interp_sact (sigma := sigma) REnv r (simplify_vars vvs) a v)
+           t (WTS: wt_sact (Sigma := Sigma) R vvs a t),
+      interp_sact (sigma := sigma) REnv r vvs a v.
+  Proof.
+    induction 3; simpl; intros; inv WTS.
+    - setoid_rewrite PTree.gmap in H. setoid_rewrite H1 in H. simpl in H. inv H.
+      econstructor; eauto.
+      eapply simplify_sact_interp_sact_ok; eauto.
+      eapply IHEV_INIT.
+      eapply wt_simplify_sact; eauto.
+    - econstructor.
+    - econstructor. eauto.
+      eapply IHEV_INIT2. destr; eauto.
+    - econstructor; eauto.
+    - econstructor; eauto.
+    - econstructor; eauto.
+    - econstructor; eauto.
+  Qed.
+
+  Lemma simplify_vars_reachable_var_ok:
+    forall vvs v (VVSSV: vvs_smaller_variables vvs) a,
+    reachable_var (simplify_vars vvs) a v
+    -> reachable_var vvs a v.
+  Proof.
+    induction 2; simpl; intros; eauto.
+    - econstructor.
+    - setoid_rewrite PTree.gmap in H. unfold option_map in H.
+      repeat destr_in H; inv H.
+      econstructor; eauto.
+      eapply simplify_sact_reachable_vars_ok. auto.
+    - eapply reachable_var_if_cond; eauto.
+    - eapply reachable_var_if_true; eauto.
+    - eapply reachable_var_if_false; eauto.
+    - eapply reachable_var_binop1; eauto.
+    - eapply reachable_var_binop2; eauto.
+    - eapply reachable_var_unop; eauto.
+    - constructor; auto.
+  Qed.
 
   Lemma sf_eq_simplify_sf sf:
     wf_sf sf -> sf_eq R Sigma r sigma sf (simplify_sf sf).
@@ -63,8 +987,8 @@ Section Simplify.
 
   Lemma simplify_sf_interp_cycle_ok:
     forall reg sf,
-    wf_sf sf ->
-    getenv REnv (interp_cycle r sigma sf) reg
+    wf_sf sf
+    -> getenv REnv (interp_cycle r sigma sf) reg
     = getenv REnv (interp_cycle r sigma (simplify_sf sf)) reg.
   Proof.
     intros.
